refactored
iptrule_match now datatype new
trying to generalize the formatting

Packet_Set.thy
@@ -18,7 +18,8 @@ fun to_negation_type_nnf :: "'a match_expr \<Rightarrow> 'a negation_type list" 
  "to_negation_type_nnf (MatchAnd a b) = (to_negation_type_nnf a) @ (to_negation_type_nnf b)"
 
 
-lemma x:"matches \<gamma> (negation_type_to_match_expr (as @ bs)) a p = matches \<gamma> (MatchAnd (negation_type_to_match_expr as) (negation_type_to_match_expr bs)) a p"
+lemma negation_type_to_match_expr_app: "matches \<gamma> (negation_type_to_match_expr (as @ bs)) a p \<longleftrightarrow>
+         matches \<gamma> (MatchAnd (negation_type_to_match_expr as) (negation_type_to_match_expr bs)) a p"
   apply(induction as arbitrary: bs)
    apply(simp_all add: bunch_of_lemmata_about_matches)
    apply(case_tac aa)
@@ -27,7 +28,7 @@ lemma x:"matches \<gamma> (negation_type_to_match_expr (as @ bs)) a p = matches 
 
 lemma "normalized_match m \<Longrightarrow> matches \<gamma> (negation_type_to_match_expr (to_negation_type_nnf m)) a p  = matches \<gamma> m a p"
   apply(induction m rule: to_negation_type_nnf.induct)
-  apply(simp_all add: bunch_of_lemmata_about_matches x)
+  apply(simp_all add: bunch_of_lemmata_about_matches negation_type_to_match_expr_app)
   done
   
   
@@ -37,6 +38,7 @@ definition to_negation_type :: "'a match_expr \<Rightarrow> ('a negation_type li
  "to_negation_type m = map to_negation_type_nnf (normalize_match m)"
 
 term normalize_match
+term normalized_match
 thm normalized_match_normalize_match
 
 
@@ -45,5 +47,67 @@ thm normalized_match_normalize_match
 definition to_packet_set :: "('a, 'packet) match_tac \<Rightarrow> action \<Rightarrow> ('a negation_type list) list \<Rightarrow> 'packet set" where
   "to_packet_set \<gamma> a ms \<equiv> {p. \<exists> m \<in> set ms. matches \<gamma> (negation_type_to_match_expr m) a p}"
 
+
+
+(*TODO create a output_format directory*)
+
+text{*
+  The following function takes a tuple of functions and a match expression.
+  The passed function tuple must be the discriminator and selector of the datatype package.
+  It filters the latter and returns a tuple.
+  The first element are the filtered primitive matches, the second element is the remaining match expression.
+  }*}
+fun primitive_extractor :: "(('a \<Rightarrow> bool) \<times> ('a \<Rightarrow> 'b)) \<Rightarrow> 'a match_expr \<Rightarrow> ('b negation_type list \<times> 'a match_expr)" where
+ "primitive_extractor _ MatchAny = ([], MatchAny)" |
+ "primitive_extractor (disc,sel) (Match a) = (if disc a then ([Pos (sel a)], MatchAny) else ([], Match a))" |
+ "primitive_extractor (disc,sel) (MatchNot (Match a)) = (if disc a then ([Neg (sel a)], MatchAny) else ([], MatchNot (Match a)))" |
+ "primitive_extractor C (MatchAnd ms1 ms2) = (
+        let (a1', ms1') = primitive_extractor C ms1; 
+            (a2', ms2') = primitive_extractor C ms2
+        in (a1'@a2', MatchAnd ms1' ms2'))"
+
+
+
+fun wf_disc_sel :: "(('a \<Rightarrow> bool) \<times> ('a \<Rightarrow> 'b)) \<Rightarrow> ('b \<Rightarrow> 'a) \<Rightarrow> bool" where
+  "wf_disc_sel (disc, sel) C = (\<forall>a. disc a \<longrightarrow> C (sel a) = a)"
+declare wf_disc_sel.simps[simp del]
+
+lemma primitive_extractor_correct: "normalized_match m \<Longrightarrow> (as, ms) = primitive_extractor (disc, sel) m \<Longrightarrow> wf_disc_sel (disc, sel) C \<Longrightarrow>
+  matches \<gamma> (negation_type_to_match_expr (NegPos_map C as)) a p \<and> matches \<gamma> ms a p \<longleftrightarrow> matches \<gamma> m a p"
+  apply(induction "(disc, sel)" m  arbitrary: as ms rule: primitive_extractor.induct)
+  apply(simp_all add: bunch_of_lemmata_about_matches wf_disc_sel.simps split: split_if_asm)
+  apply(simp split: split_if_asm split_split_asm add: NegPos_map_append)
+  apply(auto simp add: negation_type_to_match_expr_app bunch_of_lemmata_about_matches)
+  done
+
+
+(*
+text{*
+  The following function takes a filter function @{text f} and a match expression.
+  It filters the latter and returns a tuple.
+  The first element are the filtered primitive matches, the second element is the remaining match expression.
+  }*}
+fun primitive_extractor :: "('a \<Rightarrow> bool) \<Rightarrow> 'a match_expr \<Rightarrow> ('a negation_type list \<times> 'a match_expr)" where
+ "primitive_extractor _ MatchAny = ([], MatchAny)" |
+ "primitive_extractor f (Match a) = (if f a then ([Pos a], MatchAny) else ([], Match a))" |
+ "primitive_extractor f (MatchNot (Match a)) = (if f a then ([Neg a], MatchAny) else ([], MatchNot (Match a)))" |
+ "primitive_extractor f (MatchAnd ms1 ms2) = (
+        let (a1', ms1') = primitive_extractor f ms1; 
+            (a2', ms2') = primitive_extractor f ms2
+        in (a1'@a2', MatchAnd ms1' ms2'))"
+
+
+lemma primitive_extractor_correct: "normalized_match m \<Longrightarrow> (as, ms) = primitive_extractor f m \<Longrightarrow> 
+  matches \<gamma> (negation_type_to_match_expr as) a p \<and> matches \<gamma> ms a p \<longleftrightarrow> matches \<gamma> m a p"
+  apply(induction f m  arbitrary: as ms rule: primitive_extractor.induct)
+  apply(simp_all add: bunch_of_lemmata_about_matches split: split_if_asm)
+  apply(simp split: split_if_asm split_split_asm)
+  apply(auto simp add: negation_type_to_match_expr_app bunch_of_lemmata_about_matches)
+  done
+
+corollary primitive_extractor_correct': "normalized_match m  \<Longrightarrow> 
+  matches \<gamma> (negation_type_to_match_expr (fst (primitive_extractor f m))) a p \<and> matches \<gamma> (snd (primitive_extractor f m)) a p \<longleftrightarrow> matches \<gamma> m a p"
+  by(drule primitive_extractor_correct) auto
+*)
 
 end
